TODO Finish exception

2016/Exceptions.thy
@@ -3,8 +3,12 @@ imports Main "$AFP/List-Index/List_Index"
 
 begin
 
+
+
 datatype ltype=
-Unit | Fun ltype ltype (infixr "\<rightarrow>"  225)
+Unit | Fun ltype ltype (infixr "\<rightarrow>"  225) | VariantType "string list" "ltype list"("<(_):=(_)>" [201,200]225) |
+Ty string
+
 
 datatype lterm=
   LVar nat 
@@ -12,27 +16,23 @@ datatype lterm=
 | LAbs ltype lterm 
 | unit
 | error
-| trapp lterm lterm ("try/ (_)/ with/ (_)" [181,180]220)
-| raise lterm
+
 
 fun shift_L :: "int \<Rightarrow> nat \<Rightarrow> lterm \<Rightarrow> lterm" where
  "shift_L d c (LVar k)    = LVar (if k < c then k else nat (int k + d))" |
  "shift_L d c (LApp t t1) = LApp (shift_L d c t) (shift_L d c t1)" |
  "shift_L d c (LAbs T t)  = LAbs T (shift_L d (Suc c) t)" |
  "shift_L d c error = error" |
- "shift_L d c unit = unit" |
- "shift_L d c (try t with t1) = try (shift_L d c t) with (shift_L d c t1)"|
- "shift_L d c (raise t) = raise (shift_L d c t)"
+ "shift_L d c unit = unit" 
+
 
 fun subst_L :: "nat \<Rightarrow> lterm \<Rightarrow> lterm \<Rightarrow> lterm" where
  "subst_L j s (LApp t1 t2) = LApp (subst_L j s t1) (subst_L j s t2)" |
  "subst_L j s (LVar k) = (if k = j then s else LVar k)" |
  "subst_L j s (LAbs T t) = LAbs T (subst_L (Suc j) (shift_L 1 0 s) t)"|
  "subst_L j s unit = unit" |
- "subst_L j s (error) = error"|
- "subst_L j s (try t with t1) = try (subst_L j s t) with (subst_L j s t1)"|
- "subst_L j s (raise t) = raise (subst_L j s t)"
- 
+ "subst_L j s (error) = error"
+
 inductive is_value_L :: "lterm \<Rightarrow> bool" where
   "is_value_L unit"|
   "is_value_L (LAbs T t)"
@@ -50,24 +50,8 @@ inductive eval1_L :: "lterm \<Rightarrow> lterm \<Rightarrow> bool" where
   eval1_LErrApp1:
     "eval1_L (LApp error t) error"|
   eval1_LErrApp2:
-    "is_value_L v \<Longrightarrow> eval1_L (LApp v error) error" |
-  eval1_LTryV:
-    "is_value_L v \<Longrightarrow> eval1_L (try v with t) v" |
-  eval1_LTryE:
-    "eval1_L t1 t2 \<Longrightarrow> eval1_L (try t1 with t) (try t2 with t)"|
-  eval1_LTryErr:
-    "eval1_L (try error with t) t"|
-  eval1_LAppRaise1:
-    "is_value_L v \<Longrightarrow> eval1_L (LApp (raise v) t) (raise v)"|
-  eval1_LAppRaise2:
-    "is_value_L v \<Longrightarrow> is_value_L v1 \<Longrightarrow> eval1_L (LApp v (raise v1)) (raise v1)"|
-  eval1_RaiseE:
-    "eval1_L t t1 \<Longrightarrow> eval1_L (raise t) (raise t1)"|
-  eval1_RaiseRaise:
-    "is_value_L v \<Longrightarrow> eval1_L (raise (raise v)) (raise v)"|
-  eval1_TryRaise:
-    "is_value_L v \<Longrightarrow> eval1_L (try (raise v) with t2) (LApp t2 v)"
-  
+    "is_value_L v \<Longrightarrow> eval1_L (LApp v error) error" 
+ 
   
 
 type_synonym lcontext = "ltype list"
@@ -80,7 +64,7 @@ abbreviation elem' :: "(nat \<times> ltype) \<Rightarrow> lcontext \<Rightarrow>
   "elem' p \<Gamma> \<equiv> fst p < length \<Gamma> \<and> snd p = nth \<Gamma> (fst p)"
 
 
-inductive has_type_L :: "lcontext \<Rightarrow> lterm \<Rightarrow> ltype \<Rightarrow> bool" ("((_)/ \<turnstile> (_)/ |:| (_))" [150, 150, 150] 150) where
+inductive  has_type_L :: "lcontext \<Rightarrow> lterm \<Rightarrow> ltype \<Rightarrow> bool" ("((_)/ \<turnstile> (_)/ |:| (_))" [150, 150, 150] 150) where
   has_type_Lunit:
     "\<Gamma> \<turnstile> unit |:| Unit" |
   has_type_LVar:
@@ -90,10 +74,8 @@ inductive has_type_L :: "lcontext \<Rightarrow> lterm \<Rightarrow> ltype \<Righ
   has_type_LApp:
     "\<Gamma> \<turnstile> t1 |:| (T11 \<rightarrow> T12) \<Longrightarrow> \<Gamma> \<turnstile> t2 |:| T11 \<Longrightarrow> \<Gamma> \<turnstile> (LApp t1 t2) |:| T12" |
   has_type_error:
-    "\<Gamma> \<turnstile> error |:| T"|
-  has_type_try:
-    "\<Gamma> \<turnstile> t1 |:| T \<Longrightarrow> \<Gamma> \<turnstile> t2 |:| T \<Longrightarrow> \<Gamma> \<turnstile> try t1 with t2 |:| T"
-
+    "\<Gamma> \<turnstile> error |:| T"
+  
 lemma canonical_forms:
   "is_value_L v \<Longrightarrow> \<Gamma> \<turnstile> v |:| Unit \<Longrightarrow> v = unit"
   "is_value_L v \<Longrightarrow> \<Gamma> \<turnstile> v |:| T1 \<rightarrow> T2 \<Longrightarrow> \<exists>t. v = LAbs T1 t"
@@ -104,22 +86,131 @@ primrec FV :: "lterm \<Rightarrow> nat set" where
  "FV error = {}" |
  "FV (LVar x) = {x}" |
  "FV (LAbs T t) = image (\<lambda>x. x - 1) (FV t - {0})" |
- "FV (LApp t1 t2) = FV t1 \<union> FV t2"|
- "FV (try t with t1) = FV t \<union> FV t1"|
- "FV (raise t) = FV t"
+ "FV (LApp t1 t2) = FV t1 \<union> FV t2" 
 
 definition is_closed :: "lterm \<Rightarrow> bool" where
   "is_closed t \<equiv> FV t = {}"
 
 (* 14.1.2 with try and raise structure*)
 theorem progress:
-   "\<emptyset> \<turnstile> t |:| T \<Longrightarrow> is_closed t \<Longrightarrow> (\<forall>t'.\<not> eval1_L t t') \<Longrightarrow> is_value_L t \<or> t=error \<or> 
-                                      (\<exists>t1 t2. t=try t1 with t2)"
+   "\<emptyset> \<turnstile> t |:| T \<Longrightarrow> is_closed t \<Longrightarrow> (\<forall>t'.\<not> eval1_L t t') \<Longrightarrow> is_value_L t \<or> t=error"
 proof (induction t T rule: has_type_L.induct)
   case (has_type_LApp \<Gamma> t1 T11 T12 t2)
-    thus ?case sorry
-    (*by (cases "is_value_L t1", cases "is_value_L t2")
-      (auto intro: eval1_L.intros dest: canonical_forms simp: is_closed_def)*)
+    thus ?case 
+      by (cases "is_value_L t1", cases "is_value_L t2")
+          (auto intro: eval1_L.intros dest: canonical_forms simp: is_closed_def)
 qed (simp_all add: is_value_L.intros is_closed_def)
+
+
+datatype lterm1=
+  LVar1 nat 
+| LApp1 lterm1 lterm1 
+| LAbs1 ltype "string list" "ltype list" lterm1 ("LAbs1/ (_)/ <(_):=(_)>/ (_)" [200,201,200,200] 220)
+| unit1
+| trapp lterm1 lterm1 ("try/ (_)/ with/ (_)" [181,180]220)
+| raise lterm1
+| N nat
+| S string
+| Variant string lterm1 ("<(_)::=(_)>" [201,200] 220)
+
+fun shift_L1 :: "int \<Rightarrow> nat \<Rightarrow> lterm1 \<Rightarrow> lterm1" where
+ "shift_L1 d c (LVar1 k)    = LVar1 (if k < c then k else nat (int k + d))" |
+ "shift_L1 d c (LApp1 t t1) = LApp1 (shift_L1 d c t) (shift_L1 d c t1)" |
+ "shift_L1 d c (LAbs1 T <L:=TL> t)  = LAbs1 T <L:=TL> (shift_L1 d (Suc c) t)" |
+ "shift_L1 d c unit1 = unit1" |
+ "shift_L1 d c (try t with t1) = try (shift_L1 d c t) with (shift_L1 d c t1)"|
+ "shift_L1 d c (raise t) = raise (shift_L1 d c t)"|
+ "shift_L1 d c (<s::=t>) = <s::=(shift_L1 d c t)>"|
+ "shift_L1 d c t = t"
+
+fun subst_L1 :: "nat \<Rightarrow> lterm1 \<Rightarrow> lterm1 \<Rightarrow> lterm1" where
+ "subst_L1 j s (LApp1 t1 t2) = LApp1 (subst_L1 j s t1) (subst_L1 j s t2)" |
+ "subst_L1 j s (LVar1 k) = (if k = j then s else LVar1 k)" |
+ "subst_L1 j s (LAbs1 T <L:=TL> t) = LAbs1 T <L:=TL> (subst_L1 (Suc j) (shift_L1 1 0 s) t)"|
+ "subst_L1 j s unit1 = unit1" |
+ "subst_L1 j s (try t with t1) = try (subst_L1 j s t) with (subst_L1 j s t1)"|
+ "subst_L1 j s (raise t) = raise (subst_L1 j s t)"|
+ "subst_L1 j s (<s1::=t>) = <s1::=(subst_L1 j s t)>"|
+ "subst_L1 j s t = t"
+
+primrec FV1 :: "lterm1 \<Rightarrow> nat set" where
+ "FV1 unit1 = {}" |
+ "FV1 (LVar1 x) = {x}" |
+ "FV1 (LAbs1 T <L:=TL> t) = image (\<lambda>x. x - 1) (FV1 t - {0})" |
+ "FV1 (LApp1 t1 t2) = FV1 t1 \<union> FV1 t2"|
+ "FV1 (try t with t1) = FV1 t \<union> FV1 t1"|
+ "FV1 (raise t) = FV1 t"|
+ "FV1 (<s::=t>) = FV1 t"|
+ "FV1 (N _) = {}"|
+ "FV1 (S _) = {}"
+
+inductive is_value_L1 :: "lterm1 \<Rightarrow> bool" where
+  "is_value_L1 unit1"|"is_value_L1 (N _)"|"is_value_L1 (S _)"|
+  "is_value_L1 (LAbs1 T <L:=TL> t)" 
+  |"is_value_L1 v \<Longrightarrow> is_value_L1 (<s::=v>)"
+
+
+inductive eval1_L1 :: "lterm1 \<Rightarrow> lterm1 \<Rightarrow> bool" where
+  -- "Rules relating to the evaluation of function application"
+  eval1_L1App1:
+    "eval1_L1 t1 t1' \<Longrightarrow> eval1_L1 (LApp1 t1 t2) (LApp1 t1' t2)" |
+  eval1_L1App2:
+    "is_value_L1 v1 \<Longrightarrow> eval1_L1 t2 t2' \<Longrightarrow> eval1_L1 (LApp1 v1 t2) (LApp1 v1 t2')" |
+  eval1_L1App_LAbs:
+    "is_value_L1 v2 \<Longrightarrow> eval1_L1 (LApp1 (LAbs1 T <L:=TL> t12) v2)
+      (shift_L1 (-1) 0 (subst_L1 0 (shift_L1 1 0 v2) t12))" |
+  eval1_VE:
+    "eval1_L1 t t' \<Longrightarrow> eval1_L1 (<s::=t>) (<s::=t'>)"|
+  eval1_L1TryV:
+    "is_value_L1 v \<Longrightarrow> eval1_L1 (try v with t) v" |
+  eval1_L1TryE:
+    "eval1_L1 t1 t2 \<Longrightarrow> eval1_L1 (try t1 with t) (try t2 with t)"|
+  eval1_L1AppRaise1:
+    "is_value_L1 v \<Longrightarrow> eval1_L1 (LApp1 (raise v) t) (raise v)"|
+  eval1_L1AppRaise2:
+    "is_value_L1 v \<Longrightarrow> is_value_L1 v1 \<Longrightarrow> eval1_L1 (LApp1 v (raise v1)) (raise v1)"|
+  eval1_RaiseE:
+    "eval1_L1 t t1 \<Longrightarrow> eval1_L1 (raise t) (raise t1)"|
+  eval1_RaiseRaise:
+    "is_value_L1 v \<Longrightarrow> eval1_L1 (raise (raise v)) (raise v)"|
+  eval1_TryRaise:
+    "is_value_L1 v \<Longrightarrow> eval1_L1 (try (raise v) with t2) (LApp1 t2 v)"
+
+abbreviation agrees:: "lterm1 \<Rightarrow> ltype \<Rightarrow> bool" where
+ "agrees t T \<equiv> (case t of LAbs1 Ta <L:=TL> t' \<Rightarrow> (<L:=TL>)=T | _\<Rightarrow> True)"
+
+inductive  has_type1_L :: "ltype \<Rightarrow> lcontext \<Rightarrow> lterm1 \<Rightarrow> ltype \<Rightarrow> bool" ("((_)|*|(_)/ \<turnstile>\<^sub>1 (_)/ |:| (_))" [150, 150, 150] 150) where
+  has_type1_Lunit:
+    "T\<alpha>|*|\<Gamma> \<turnstile>\<^sub>1 unit1 |:| Unit" |
+  has_type1_LNat:
+    "T\<alpha>|*|\<Gamma> \<turnstile>\<^sub>1 (N n) |:| Ty ''nat''"|
+  has_type1_LString:
+    "T\<alpha>|*|\<Gamma> \<turnstile>\<^sub>1 (S s) |:| Ty ''str''"|
+  has_type1_LVar:
+    "(x, T) |\<in>| \<Gamma> \<Longrightarrow> T\<alpha>|*|\<Gamma> \<turnstile>\<^sub>1 (LVar1 x) |:| T" |
+  has_type1_LAbs:
+    "distinct L \<Longrightarrow> agrees t2 (<L:=TL>) \<Longrightarrow> <L:=TL>|*|(\<Gamma> |,| T1) \<turnstile>\<^sub>1 t2 |:| T2 \<Longrightarrow> T\<alpha>1|*|\<Gamma> \<turnstile>\<^sub>1 (LAbs1 T1 <L:=TL> t2) |:| (T1 \<rightarrow> T2)" |
+  has_type1_LApp:
+    "T\<alpha>|*|\<Gamma> \<turnstile>\<^sub>1 t1 |:| (T11 \<rightarrow> T12) \<Longrightarrow> T\<alpha>|*|\<Gamma> \<turnstile>\<^sub>1 t2 |:| T11 \<Longrightarrow> T\<alpha>|*|\<Gamma> \<turnstile>\<^sub>1 (LApp1 t1 t2) |:| T12" |
+  has_type1_Variant:
+    "L!i = s \<Longrightarrow> TL!i= A \<Longrightarrow> T\<alpha>|*|\<Gamma> \<turnstile>\<^sub>1 t |:| A \<Longrightarrow>T\<alpha>|*|\<Gamma> \<turnstile>\<^sub>1 <s::=t> |:| <L:=TL>" |
+  has_type1_try:
+    "T\<alpha>|*|\<Gamma> \<turnstile>\<^sub>1 t1 |:| T \<Longrightarrow> T\<alpha>|*|\<Gamma> \<turnstile>\<^sub>1 t2 |:| T\<alpha>\<rightarrow>T \<Longrightarrow> T\<alpha>|*|\<Gamma> \<turnstile>\<^sub>1 try t1 with t2 |:| T" |
+  has_type1_raise:
+    "T\<alpha>|*|\<Gamma> \<turnstile>\<^sub>1 t |:| T\<alpha> \<Longrightarrow> T\<alpha>|*|\<Gamma> \<turnstile>\<^sub>1 raise t |:| T"
+
+lemma canonical_forms1:
+  "is_value_L1 v \<Longrightarrow> T\<alpha>|*|\<Gamma> \<turnstile>\<^sub>1 v |:| Unit \<Longrightarrow> v = unit1"
+  "is_value_L1 v \<Longrightarrow> T\<alpha>|*|\<Gamma> \<turnstile>\<^sub>1 v |:| T1 \<rightarrow> T2 \<Longrightarrow> \<exists>t L TL. v = LAbs1 T1 <L:=TL> t"
+by (auto elim: "is_value_L1.cases" has_type1_L.cases)
+
+lemma progress1:
+  "<\<emptyset>:=\<emptyset>>|*|\<emptyset> \<turnstile>\<^sub>1 t |:| T \<Longrightarrow> is_value_L1 t \<or> (\<exists>t'. eval1_L1 t t')"
+sorry
+
+
+lemma preservation:
+  "T\<alpha>|*|\<Gamma> \<turnstile>\<^sub>1 t |:| T \<Longrightarrow> eval1_L1 t t' \<Longrightarrow> T\<alpha>|*|\<Gamma> \<turnstile>\<^sub>1 t' |:| T"
+sorry
 
 end
